SecurityExamples.v
@@ -1,0 +1,56 @@
+Require Import Arith Process Refinement ModelCheck.
+
+
+Definition chs : channels := fun _ => nat.
+
+(* Policy: Process may only send on channel "out". *)
+Module SendOnlyOnOut.
+  Definition policy (pr : process chs) : process chs :=
+    ##[(Send, "out")], pr.
+
+  Definition impl : process chs :=
+    #!chs["out", 1], Done.
+
+  Theorem conforms : exists pr, refines impl (policy pr).
+  Proof.
+    exists impl.
+    refines.
+    refines.
+  Qed.
+End SendOnlyOnOut.
+
+(* Policy: Process should only send a number less than or equal to 5. *)
+Module SendLe5.
+  Definition policy (pr : process chs) : process chs :=
+    (##[(Send, "tmp")], pr) || (#?chs["tmp", n], if leb n 5 then #!chs["out", n], Done else Done).
+
+  Definition impl : process chs :=
+    #!chs["out", 4], Done.
+
+  Theorem conforms : exists pr, refines impl (policy pr).
+  Proof.
+    exists (#!chs["tmp", 4], Done).
+    refines.
+    refines.
+    refines.
+  Qed.
+End SendLe5.
+
+(* Policy: Process receives two numbers and is only allowed to depend on their sum. *)
+Module OnlySum.
+  Definition policy (pr : process chs) : process chs := ##[(Recv, "in"), (Send, "out")],
+    (##[(Recv, "tmp"), (Send, "out")], pr) || (#?chs["in", n], #?chs["in", m], #!chs["tmp", n + m], Done).
+
+  Definition impl : process chs :=
+    #?chs["in", n], #?chs["in", m], #!chs["out", 3 + (n + m)], Done.
+
+  Theorem conforms : exists pr, refines impl (policy pr).
+  Proof.
+    exists (#?chs["tmp", sum], #!chs["out", 3 + sum], Done).
+    refines.
+    refines.
+    refines.
+    refines.
+    refines.
+  Qed.
+End OnlySum.
